experimenting with weakest preconditions

src/crypto/poly1305/x64/X64.Poly1305.Bitvectors_i.fst
@@ -5,42 +5,42 @@ open FStar.Tactics
 open FStar.Tactics.Derived
 open FStar.Tactics.BV
 open FStar.Mul
-module U = FStar.UInt
+open FStar.UInt
 
 // tweak options?
 #reset-options "--smtencoding.elim_box true"
 
 let lemma_shr2 x = 
-   assert_by_tactic (bv_tac()) (U.shift_right #64 x 2 == U.udiv #64 x 4)
+   assert_by_tactic (bv_tac()) (shift_right #64 x 2 == udiv #64 x 4)
    
 let lemma_shr4 x =
-  assert_by_tactic (bv_tac ()) (U.shift_right #64 x 4 == U.udiv #64 x 16)
+  assert_by_tactic (bv_tac ()) (shift_right #64 x 4 == udiv #64 x 16)
 
 let lemma_and_mod_n x =
   assert_by_tactic (seq split (bv_tac ())) 
-    (U.logand #64 x 3 == U.mod #64 x 4 /\ U.logand #64 x 15 == U.mod #64 x 16)
+    (logand #64 x 3 == mod #64 x 4 /\ logand #64 x 15 == mod #64 x 16)
 
 let lemma_clear_lower_2 x =
   assert_by_tactic (bv_tac ())
-  (U.logand #8 x 0xfc == U.mul_mod #8 (U.udiv #8 x 4) 4)
+  (logand #8 x 0xfc == mul_mod #8 (udiv #8 x 4) 4)
 
 let lemma_and_constants x =
   assert_by_tactic (seq split (bv_tac ()))
-  (U.logand #64 x 0 == (0 <: uint_t' 64) /\ 
-   U.logand #64 x 0xffffffffffffffff == x)
+  (logand #64 x 0 == (0 <: uint_t 64) /\ 
+   logand #64 x 0xffffffffffffffff == x)
 
 let lemma_poly_constants x =
  assert_by_tactic (split;; split;; 
 		   bv_tac_lt 64;;
 		   bv_tac_lt 64;;
 		   bv_tac ()) 
-   (U.logand #64 x 0x0ffffffc0fffffff < (0x1000000000000000 <: uint_t' 64) /\
-     U.logand #64 x 0x0ffffffc0ffffffc < (0x1000000000000000 <: uint_t' 64) /\
-     U.mod #64 (U.logand #64 x 0x0ffffffc0ffffffc) 4 == (0 <: uint_t' 64))
+   (logand #64 x 0x0ffffffc0fffffff < (0x1000000000000000 <: uint_t 64) /\
+     logand #64 x 0x0ffffffc0ffffffc < (0x1000000000000000 <: uint_t 64) /\
+     mod #64 (logand #64 x 0x0ffffffc0ffffffc) 4 == (0 <: uint_t 64))
 
 let lemma_and_commutes x y =
   assert_by_tactic (bv_tac ())
-    (U.logand #64 x y == U.logand #64 y x)
+    (logand #64 x y == logand #64 y x)
 
 let lemma_bv128_64_64_and_helper x x0 x1 y y0 y1 z z0 z1 =
   ()
@@ -51,67 +51,96 @@ let lemma_bv128_64_64_and x x0 x1 y y0 y1 z z0 z1 =
   ()
 
 
-(* is lowerUpper128 useful? *)
-// val lowerUpper128: l:uint_t' 64 -> u:uint_t' 64 -> Tot (uint_t' 128)
-// let lowerUpper128 l u = l + (0x10000000000000000 * u)
+// is lowerUpper128 useful?
+val lowerUpper128: l:uint_t 64 -> u:uint_t 64 -> Tot (uint_t 128)
+let lowerUpper128 l u = l + (0x10000000000000000 * u)
 
-// val lemma_lowerUpper128_and: x:uint_t' 128 -> x0:uint_t' 64 -> x1:uint_t' 64 ->
-//   y:uint_t' 128 -> y0:uint_t' 64 -> y1:uint_t' 64 ->
-//   z:uint_t' 128 -> z0:uint_t' 64 -> z1:uint_t' 64 ->
-//   Lemma (requires (z0 == U.logand #64 x0 y0 /\
-// 		   z1 == U.logand #64 x1 y1 /\
-// 		   x == lowerUpper128 x1 x0 /\
-// 		   y == lowerUpper128 y1 y0 /\
-// 		   z == lowerUpper128 z1 z0))
-// 	(ensures (z == U.logand #128 x y))
-// let lemma_lowerUpper128_and x x0 x1 y y0 y1 z z0 z1 =
-  
+val lemma_lowerUpper128_and: x:uint_t 128 -> x0:uint_t 64 -> x1:uint_t 64 ->
+  y:uint_t 128 -> y0:uint_t 64 -> y1:uint_t 64 ->
+  z:uint_t 128 -> z0:uint_t 64 -> z1:uint_t 64 ->
+  Lemma (requires (z0 == logand #64 x0 y0 /\
+		   z1 == logand #64 x1 y1 /\
+		   x == lowerUpper128 x1 x0 /\
+		   y == lowerUpper128 y1 y0 /\
+		   z == lowerUpper128 z1 z0))
+	(ensures (z == logand #128 x y))
+let lemma_lowerUpper128_and x x0 x1 y y0 y1 z z0 z1 = ()
 
-let lemma_bytes_shift_constants () =
-  assert_by_tactic (seq split (bv_tac()))
-    (U.shift_left #64 0 3 == 0 /\
-      U.shift_left #64 1 3 == 8);
-  assert_by_tactic (seq split (bv_tac()))
-      (U.shift_left #64 2 3 == 16 /\
-       U.shift_left #64 3 3 == 24);
-  assert_by_tactic (seq split (bv_tac()))
-    (U.shift_left #64 4 3 == 32 /\
-     U.shift_left #64 5 3 == 40);
-  assert_by_tactic (seq split (bv_tac()))
-    (U.shift_left #64 6 3 == 48 /\
-      U.shift_left #64 7 3 == 56);
-  assert_by_tactic (seq split (bv_tac()))
-  (U.shift_left #64 1 0 == 0x1 /\
-    U.shift_left #64 1 8 == 0x100);
-  assert_by_tactic (seq split (bv_tac()))
-    (U.shift_left #64 1 16 == 0x10000 /\
-      U.shift_left #64 1 24 == 0x1000000);
-  assert_by_tactic (seq split (bv_tac()))
-    (U.shift_left #64 1 32 == 0x100000000 /\
-      U.shift_left #64 1 40 == 0x10000000000);
-  assert_by_tactic (seq split (bv_tac()))
-    (U.shift_left #64 1 48 == 0x1000000000000 /\
-      U.shift_left #64 1 56 == 0x100000000000000);
-  ()
+#reset-options "--smtencoding.elim_box true --z3rlimit_factor 2 --z3cliopt smt.case_split=3"
+let lemma_bytes_shift_constants0 x =
+  assert_by_tactic (bv_tac())
+    (shift_left #64 0 3 == (0 <: uint_t 64));
+  assert_by_tactic (bv_tac())
+    (shift_left #64 1 0 == (0x1 <: uint_t 64))
+let lemma_bytes_shift_constants1 x =
+  assert_by_tactic (bv_tac())
+    (shift_left #64 1 3 == (8 <: uint_t 64));
+  assert_by_tactic (bv_tac())
+    (shift_left #64 1 8 == (0x100 <: uint_t 64))
+let lemma_bytes_shift_constants2 x =
+  assert_by_tactic (bv_tac())
+    (shift_left #64 2 3 == (16 <: uint_t 64));
+  assert_by_tactic (bv_tac())
+    (shift_left #64 1 16 == (0x10000 <: uint_t 64))
+let lemma_bytes_shift_constants3 x =
+  assert_by_tactic (bv_tac())
+    (shift_left #64 3 3 == (24 <: uint_t 64));
+  assert_by_tactic (bv_tac())
+    (shift_left #64 1 24 == (0x1000000 <: uint_t 64))
+let lemma_bytes_shift_constants4 x =
+  assert_by_tactic (bv_tac())
+    (shift_left #64 4 3 == (32 <: uint_t 64));
+    assert_by_tactic (bv_tac())
+    (shift_left #64 1 32 == (0x100000000 <: uint_t 64))
+let lemma_bytes_shift_constants5 x =
+  assert_by_tactic (bv_tac())
+    (shift_left #64 5 3 == (40 <: uint_t 64));
+  assert_by_tactic (bv_tac())
+    (shift_left #64 1 40 == (0x10000000000 <: uint_t 64))
+let lemma_bytes_shift_constants6 x =
+  assert_by_tactic (bv_tac())
+    (shift_left #64 6 3 == (48 <: uint_t 64));
+  assert_by_tactic (bv_tac())
+    (shift_left #64 1 48 == (0x1000000000000 <: uint_t 64))   
+let lemma_bytes_shift_constants7 x =
+  assert_by_tactic (bv_tac())
+    (shift_left #64 7 3 == (56 <: uint_t 64)); 
+  assert_by_tactic (bv_tac())
+    (shift_left #64 1 56 == (0x100000000000000 <: uint_t 64))
 
-let lemma_bytes_and_mod0 x = ()
+let lemma_bytes_and_mod0 x = 
+  assert_by_tactic (bv_tac ()) (logand #64 x (0x1 - 1) == mod #64 x 0x1)
 
-let lemma_bytes_and_mod1 x = ()
+let lemma_bytes_and_mod1 x = 
+  assert_by_tactic (bv_tac ()) (logand #64 x (0x100 - 1) == mod #64 x 0x100)
 
-let lemma_bytes_and_mod2 x = ()
+let lemma_bytes_and_mod2 x = 
+  assert_by_tactic (bv_tac ()) (logand #64 x (0x10000 - 1) == mod #64 x 0x10000)
+let lemma_bytes_and_mod3 x =
+  assert_by_tactic (bv_tac ())(logand #64 x (0x1000000 - 1) == mod #64 x 0x1000000)
 
-let lemma_bytes_and_mod3 x = ()
+let lemma_bytes_and_mod4 x = 
+  assert_by_tactic (bv_tac ()) (logand #64 x (0x100000000 - 1) == mod #64 x 0x100000000)
 
-let lemma_bytes_and_mod4 x = ()
+let lemma_bytes_and_mod5 x = 
+  assert_by_tactic (bv_tac ()) (logand #64 x (0x10000000000 - 1) == mod #64 x 0x10000000000)
 
-let lemma_bytes_and_mod5 x = ()
+let lemma_bytes_and_mod6 x = 
+  assert_by_tactic (bv_tac ()) (logand #64 x (0x1000000000000 - 1) == mod #64 x 0x1000000000000)
 
-let lemma_bytes_and_mod6 x = ()
+let lemma_bytes_and_mod7 x = 
+  assert_by_tactic (bv_tac ()) 
+    (logand #64 x (0x100000000000000 - 1) == mod #64 x 0x100000000000000)
 
-let lemma_bytes_and_mod7 x = ()
-
-let lemma_bytes_and_mod_bv x y z =
-    lemma_bytes_shift_constants ();
+let lemma_bytes_and_mod x y =
+    lemma_bytes_shift_constants0 ();
+    lemma_bytes_shift_constants1 ();
+    lemma_bytes_shift_constants2 ();
+    lemma_bytes_shift_constants3 ();
+    lemma_bytes_shift_constants4 ();
+    lemma_bytes_shift_constants5 ();
+    lemma_bytes_shift_constants6 ();
+    lemma_bytes_shift_constants7 ();
     lemma_bytes_and_mod0 x;
     lemma_bytes_and_mod1 x;
     lemma_bytes_and_mod2 x;
@@ -119,23 +148,7 @@ let lemma_bytes_and_mod_bv x y z =
     lemma_bytes_and_mod4 x;
     lemma_bytes_and_mod5 x;
     lemma_bytes_and_mod6 x;
-    lemma_bytes_and_mod7 x;
-    ()
-
-// val lemma_bytes_and_mod: x: bv_t 64 -> y:bv_t 64 -> z:bv_t 64 ->
-//   Lemma (requires (bvult #64 y (int2bv #64 8) /\
-//   		   z == bvshl #64 (int2bv #64 1) (bv2int (bvshl y 3))))
-// 	 (ensures (z <> bv_zero #64 /\ bvult #64 (bvshl y 3) (int2bv #64 64)))
-// let lemma_bytes_and_mod_bv x y z =
-//     lemma_bytes_and_mod0 x;
-//     lemma_bytes_and_mod1 x;
-//     lemma_bytes_and_mod2 x;
-//     lemma_bytes_and_mod3 x;
-//     lemma_bytes_and_mod4 x;
-//     lemma_bytes_and_mod5 x;
-//     lemma_bytes_and_mod6 x;
-//     lemma_bytes_and_mod7 x;
-//     ()
+    lemma_bytes_and_mod7 x; ()
 
 let lemma_bytes_power2 () =
   assert_norm (pow2 0 == 0x1);
@@ -149,9 +162,13 @@ let lemma_bytes_power2 () =
   ()
 
 let lemma_bytes_shift_power2 y =
-  // assert_by_tactic (bv_tac_lt 64) (U.shift_left #64 y 3 < (64 <: uint_t' 64));
-  // assert_by_tactic (bv_tac ()) (y * 8 == U.shift_left #64 y 3);
-    assume (U.shift_left #64 y 3 < (64 <: uint_t' 64));
-    assume (y * 8 == U.shift_left #64 y 3);
-    lemma_bytes_shift_constants ();
+    lemma_bytes_shift_constants0 ();
+    lemma_bytes_shift_constants1 ();
+    lemma_bytes_shift_constants2 ();
+    lemma_bytes_shift_constants3 ();
+    lemma_bytes_shift_constants4 ();
+    lemma_bytes_shift_constants5 ();
+    lemma_bytes_shift_constants6 ();
+    lemma_bytes_shift_constants7 ();
     lemma_bytes_power2 ()
+
