src/crypto/poly1305/x64/X64.Poly1305.Bitvectors_i.fsti
@@ -2,24 +2,24 @@ module X64.Poly1305.Bitvectors_i
 
 open FStar.BV
 open FStar.Mul
-module U = FStar.UInt
+open FStar.UInt
 
-val lemma_shr2: x:uint_t' 64 -> Lemma (U.shift_right #64 x 2 == U.udiv #64 x 4)
-val lemma_shr4: x:uint_t' 64 -> Lemma (U.shift_right #64 x 4 == U.udiv #64 x 16)
+val lemma_shr2: x:uint_t 64 -> Lemma (shift_right #64 x 2 == udiv #64 x 4)
+val lemma_shr4: x:uint_t 64 -> Lemma (shift_right #64 x 4 == udiv #64 x 16)
 
-val lemma_and_mod_n: x:uint_t' 64 -> Lemma (U.logand #64 x 3 == U.mod #64 x 4 /\ 
-				      U.logand #64 x 15 == U.mod #64 x 16)
-val lemma_clear_lower_2: x:uint_t' 8 -> Lemma (U.logand #8 x 0xfc == 
-					U.mul_mod #8 (U.udiv #8 x 4) 4)
-val lemma_and_constants: x:uint_t' 64 ->
-  Lemma (U.logand #64 x 0 == 0 /\ U.logand #64 x 0xffffffffffffffff == x)
-val lemma_poly_constants: x:uint_t' 64 -> 
-  Lemma (U.logand #64 x 0x0ffffffc0fffffff < 0x1000000000000000 /\
-	 U.logand #64 x 0x0ffffffc0ffffffc < 0x1000000000000000 /\
-	 U.mod #64 (U.logand #64 x 0x0ffffffc0ffffffc) 4 == 0)
+val lemma_and_mod_n: x:uint_t 64 -> Lemma (logand #64 x 3 == mod #64 x 4 /\ 
+				      logand #64 x 15 == mod #64 x 16)
+val lemma_clear_lower_2: x:uint_t 8 -> Lemma (logand #8 x 0xfc == 
+					mul_mod #8 (udiv #8 x 4) 4)
+val lemma_and_constants: x:uint_t 64 ->
+  Lemma (logand #64 x 0 == 0 /\ logand #64 x 0xffffffffffffffff == x)
+val lemma_poly_constants: x:uint_t 64 -> 
+  Lemma (logand #64 x 0x0ffffffc0fffffff < 0x1000000000000000 /\
+	 logand #64 x 0x0ffffffc0ffffffc < 0x1000000000000000 /\
+	 mod #64 (logand #64 x 0x0ffffffc0ffffffc) 4 == 0)
 	 
-val lemma_and_commutes: x:uint_t' 64 -> y:uint_t' 64 ->
-  Lemma (U.logand #64 x y == U.logand #64 y x)
+val lemma_and_commutes: x:uint_t 64 -> y:uint_t 64 ->
+  Lemma (logand #64 x y == logand #64 y x)
 val lemma_bv128_64_64_and_helper: x:bv_t 128 -> x0:bv_t 64 -> x1:bv_t 64 ->
   y:bv_t 128 -> y0:bv_t 64 -> y1:bv_t 64 ->
   z:bv_t 128 -> z0:bv_t 64 -> z1:bv_t 64 ->
@@ -41,57 +41,75 @@ val lemma_bv128_64_64_and: x:bv_t 128 -> x0:bv_t 64 -> x1:bv_t 64 ->
 		   z == bv128_64_64 z1 z0))
 	(ensures (z == bvand #128 x y))
 
-val lemma_bytes_shift_constants: unit -> Lemma
-    (ensures (U.shift_left #64 0 3 == 0 /\
-	     U.shift_left #64 1 3 == 8 /\
-	     U.shift_left #64 2 3 == 16 /\
-	     U.shift_left #64 3 3 == 24 /\
-	     U.shift_left #64 4 3 == 32 /\
-	     U.shift_left #64 5 3 == 40 /\
-	     U.shift_left #64 6 3 == 48 /\
-	     U.shift_left #64 7 3 == 56 /\
-	     U.shift_left #64 1 (U.shift_left #64 0 3) == 0x1 /\
-	     U.shift_left #64 1 (U.shift_left #64 1 3) == 0x100 /\
-	     U.shift_left #64 1 (U.shift_left #64 2 3) == 0x10000 /\
-	     U.shift_left #64 1 (U.shift_left #64 3 3) == 0x1000000 /\
-	     U.shift_left #64 1 (U.shift_left #64 4 3) == 0x100000000 /\
-	     U.shift_left #64 1 (U.shift_left #64 5 3) == 0x10000000000 /\
-	     U.shift_left #64 1 (U.shift_left #64 6 3) == 0x1000000000000 /\
-	     U.shift_left #64 1 (U.shift_left #64 7 3) == 0x100000000000000))
 
-val lemma_bytes_and_mod0: x: bv_t 64 ->
-  Lemma (bvand x (int2bv #64 (0x1 - 1)) == bvmod x 0x1)
-val lemma_bytes_and_mod1: x: bv_t 64 ->
-  Lemma (bvand x (int2bv #64 (0x100 - 1)) == bvmod x 0x100)
-val lemma_bytes_and_mod2: x: bv_t 64 ->
-  Lemma (bvand x (int2bv #64 (0x10000 - 1)) == bvmod x 0x10000)
-val lemma_bytes_and_mod3: x: bv_t 64 ->
-  Lemma (bvand x (int2bv #64 (0x1000000 - 1)) == bvmod x 0x1000000)
-val lemma_bytes_and_mod4: x: bv_t 64 ->
-  Lemma (bvand x (int2bv #64 (0x100000000 - 1)) == bvmod x 0x100000000)
-val lemma_bytes_and_mod5: x: bv_t 64 ->
-  Lemma (bvand x (int2bv #64 (0x10000000000 - 1)) == bvmod x 0x10000000000)
-val lemma_bytes_and_mod6: x: bv_t 64 ->
-  Lemma (bvand x (int2bv #64 (0x1000000000000 - 1)) == bvmod x 0x1000000000000)
-val lemma_bytes_and_mod7: x: bv_t 64 ->
-  Lemma (bvand x (int2bv #64 (0x100000000000000 - 1)) == bvmod x 0x100000000000000)
-val lemma_bytes_and_mod_bv: x: bv_t 64 -> y:bv_t 64 -> z:bv_t 64 ->
-  Lemma (requires (bvult #64 y (int2bv #64 8) /\
-	z == bvshl #64 (int2bv #64 1) (bv2int (bvshl y 3))))
-	(ensures (z <> bv_zero #64 /\ bvult #64 (bvshl y 3) (int2bv #64 64)))
+val lemma_bytes_shift_constants0: unit -> Lemma
+    (shift_left #64 0 3 == 0 /\
+	     shift_left #64 1 (shift_left #64 0 3) == 0x1)
+
+val lemma_bytes_shift_constants1: unit -> Lemma
+    (shift_left #64 1 3 == 8 /\
+	     shift_left #64 1 (shift_left #64 1 3) == 0x100)
+
+val lemma_bytes_shift_constants2: unit -> Lemma
+    (shift_left #64 2 3 == 16 /\
+	     shift_left #64 1 (shift_left #64 2 3) == 0x10000)
+
+val lemma_bytes_shift_constants3: unit -> Lemma
+    (shift_left #64 3 3 == 24 /\
+	     shift_left #64 1 (shift_left #64 3 3) == 0x1000000)
+
+val lemma_bytes_shift_constants4: unit -> Lemma
+    (shift_left #64 4 3 == 32 /\
+	     shift_left #64 1 (shift_left #64 4 3) == 0x100000000)
+
+val lemma_bytes_shift_constants5: unit -> Lemma
+    (shift_left #64 5 3 == 40 /\
+	     shift_left #64 1 (shift_left #64 5 3) == 0x10000000000)
+
+val lemma_bytes_shift_constants6: unit -> Lemma
+    (shift_left #64 6 3 == 48 /\
+	     shift_left #64 1 (shift_left #64 6 3) == 0x1000000000000)
+
+val lemma_bytes_shift_constants7: unit -> Lemma
+    (shift_left #64 7 3 == 56 /\
+	     shift_left #64 1 (shift_left #64 7 3) == 0x100000000000000)
+
+val lemma_bytes_and_mod0: x: uint_t 64 ->
+  Lemma (logand #64 x  (0x1 - 1) == mod #64 x 0x1)
+val lemma_bytes_and_mod1: x: uint_t 64 ->
+  Lemma (logand #64 x  (0x100 - 1) == mod #64 x 0x100)
+val lemma_bytes_and_mod2: x: uint_t 64 ->
+  Lemma (logand #64 x  (0x10000 - 1) == mod #64 x 0x10000)
+val lemma_bytes_and_mod3: x: uint_t 64 ->
+  Lemma (logand #64 x  (0x1000000 - 1) == mod #64 x 0x1000000)
+val lemma_bytes_and_mod4: x: uint_t 64 ->
+  Lemma (logand #64 x  (0x100000000 - 1) == mod #64 x 0x100000000)
+val lemma_bytes_and_mod5: x: uint_t 64 ->
+  Lemma (logand #64 x  (0x10000000000 - 1) == mod #64 x 0x10000000000)
+val lemma_bytes_and_mod6: x: uint_t 64 ->
+  Lemma (logand #64 x  (0x1000000000000 - 1) == mod #64 x 0x1000000000000)
+val lemma_bytes_and_mod7: x: uint_t 64 ->
+  Lemma (logand #64 x  (0x100000000000000 - 1) == mod #64 x 0x100000000000000)
+
+val lemma_bytes_and_mod: x: uint_t 64 -> y:uint_t 64 ->
+  Lemma (requires (y < 8))
+	(ensures (shift_left #64 y 3 < 64 /\ 
+		   (shift_left #64 1 (shift_left #64 y 3)) <> 0 /\ 
+		   logand #64 x (((shift_left #64 1 (shift_left #64 y 3))) - 1) == 
+		   mod #64 x (shift_left #64 1 (shift_left #64 y 3))))
 
 val lemma_bytes_power2: unit ->
 Lemma (ensures (pow2 0 == 0x1 /\
-	       pow2 8 == 0x100 /\
-		 pow2 16 == 0x10000 /\
-		 pow2 24 == 0x1000000 /\
-		 pow2 32 == 0x100000000 /\
-		 pow2 40 == 0x10000000000 /\
-		 pow2 48 == 0x1000000000000 /\
-		 pow2 56 == 0x100000000000000))
+	        pow2 8 == 0x100 /\
+		pow2 16 == 0x10000 /\
+		pow2 24 == 0x1000000 /\
+		pow2 32 == 0x100000000 /\
+		pow2 40 == 0x10000000000 /\
+		pow2 48 == 0x1000000000000 /\
+		pow2 56 == 0x100000000000000))
 
-val lemma_bytes_shift_power2: y:uint_t' 64 ->
+val lemma_bytes_shift_power2: y:uint_t 64 ->
   Lemma (requires (y < 8))
-	(ensures  (U.shift_left #64 y 3 < 64 /\
-		   y * 8 == U.shift_left #64 y 3 /\
-		   pow2 (U.shift_left #64 y 3) == U.shift_left #64 1 (U.shift_left #64 y 3)))
+	(ensures  (shift_left #64 y 3 < 64 /\
+		   y * 8 == shift_left #64 y 3 /\
+		   pow2 (shift_left #64 y 3) == shift_left #64 1 (shift_left #64 y 3)))
